abp/FairDelayAutomaton.thy
@@ -3,10 +3,10 @@
  * This file was generated from FairDelay.maa and will be overridden when changed. To change
  * permanently, consider changing the model itself.
  *
- * isartransformer 1.0.0
+ * isartransformer 2.0.0
  *)
 theory FairDelayAutomaton
-  imports FairDelayDatatype automat.ndAutomaton
+  imports FairDelayDatatype FairDelayStates automat.ndAutomaton
 
 begin
 
@@ -17,23 +17,6 @@ fun prepend :: "'a::type list \<Rightarrow> 'a \<Rightarrow> 'a list" where
 
 
 section \<open>Automaton definition\<close>
-
-(* These are the actual states from MAA *)
-datatype FairDelaySubstate = Single
-
-(* And these have also the variables *)
-datatype 'e FairDelayState = FairDelayState FairDelaySubstate (* ctr = *) "nat" (* buffer = *) "'e list"
-
-(* Function to get the substate *)
-fun getFairDelaySubState :: "'e FairDelayState \<Rightarrow> FairDelaySubstate" where
-"getFairDelaySubState (FairDelayState s _ _) = s"
-
-(* Functions to get the variables *)
-fun getCtr :: "'e FairDelayState \<Rightarrow> nat" where
-"getCtr (FairDelayState _ var_ctr var_buffer) = var_ctr"
-
-fun getBuffer :: "'e FairDelayState \<Rightarrow> 'e list" where
-"getBuffer (FairDelayState _ var_ctr var_buffer) = var_buffer"
 
 (* Helper that allows us to utilize pattern matching *)
 fun fairDelayTransitionH :: "('e FairDelayState \<times> ('e tsyn)) \<Rightarrow> ('e FairDelayState \<times> ('e::countable) fairDelayMessage tsyn SB) set rev" where
