abp/MediumAutomaton.thy
@@ -3,10 +3,10 @@
  * This file was generated from Medium.maa and will be overridden when changed. To change
  * permanently, consider changing the model itself.
  *
- * isartransformer 1.0.0
+ * isartransformer 2.0.0
  *)
 theory MediumAutomaton
-  imports MediumDatatype automat.ndAutomaton
+  imports MediumDatatype MediumStates automat.ndAutomaton
 
 begin
 
@@ -17,20 +17,6 @@ fun prepend :: "'a::type list \<Rightarrow> 'a \<Rightarrow> 'a list" where
 
 
 section \<open>Automaton definition\<close>
-
-(* These are the actual states from MAA *)
-datatype MediumSubstate = Single
-
-(* And these have also the variables *)
-datatype MediumState = MediumState MediumSubstate (* c = *) "nat"
-
-(* Function to get the substate *)
-fun getMediumSubState :: "MediumState \<Rightarrow> MediumSubstate" where
-"getMediumSubState (MediumState s _) = s"
-
-(* Functions to get the variables *)
-fun getC :: "MediumState \<Rightarrow> nat" where
-"getC (MediumState _ var_c) = var_c"
 
 (* Helper that allows us to utilize pattern matching *)
 fun mediumTransitionH :: "(MediumState \<times> ('e tsyn)) \<Rightarrow> (MediumState \<times> ('e::countable) mediumMessage tsyn SB) set rev" where
