abp/MediumStates.thy
@@ -1,0 +1,29 @@
+(*
+ * DO NOT MODIFY!
+ * This file was generated from Medium.maa and will be overridden when changed. To change
+ * permanently, consider changing the model itself.
+ *
+ * isartransformer 2.0.0
+ *)
+theory MediumStates
+  imports MediumDatatype
+
+begin
+
+
+(* These are the actual states from MAA *)
+datatype MediumSubstate = Single
+
+(* And these have also the variables *)
+datatype MediumState = MediumState MediumSubstate (* c = *) "nat"
+
+(* Function to get the substate *)
+fun getMediumSubState :: "MediumState \<Rightarrow> MediumSubstate" where
+    "getMediumSubState (MediumState s _) = s"
+
+(* Functions to get the variables *)
+fun getC :: "MediumState \<Rightarrow> nat" where
+"getC (MediumState _ var_c) = var_c"
+
+
+end
