abp/ReceiverStates.thy
@@ -1,0 +1,25 @@
+(*
+ * DO NOT MODIFY!
+ * This file was generated from Receiver.maa and will be overridden when changed. To change
+ * permanently, consider changing the model itself.
+ *
+ * isartransformer 2.0.0
+ *)
+theory ReceiverStates
+  imports ReceiverDatatype
+
+begin
+
+
+(* These are the actual states from MAA *)
+datatype ReceiverSubstate = Rf | Rt
+
+(* And these have also the variables *)
+datatype ReceiverState = ReceiverState ReceiverSubstate 
+
+(* Function to get the substate *)
+fun getReceiverSubState :: "ReceiverState \<Rightarrow> ReceiverSubstate" where
+    "getReceiverSubState (ReceiverState s ) = s"
+
+
+end
